S2I/Backward.v
@@ -1,0 +1,187 @@
+Require Import Common.Definitions.
+Require Import Common.Memory.
+Require Import CompCert.Events.
+Require Import CompCert.Smallstep.
+(* Require Import CompCert.Behaviors. *)
+Require Import Source.Language.
+Require Import Source.GlobalEnv.
+Require Import Source.PS.
+Require Import Intermediate.Machine.
+Require Import Intermediate.PS.
+Require Import S2I.Compiler.
+
+Module SP := Source.PS.PS.
+Module SC := Source.CS.CS.
+Module IP := Intermediate.PS.PS.
+Module IC := Intermediate.CS.CS.
+
+Variable prog: Source.program.
+Variable tprog: Intermediate.program.
+Hypothesis TRANSL: S2I.Compiler.compile_program prog = Some tprog.
+
+(* Definition L1 := IC.sem tprog. *)
+(* Definition L2 := SC.sem prog. *)
+
+Module Cbs.
+
+  Axiom match_stacks: IC.stack -> SC.stack -> Prop.
+  Axiom match_states: IC.state -> SC.state -> Prop.
+
+  Axiom match_initial_states:
+    forall s1, initial_state (IC.sem tprog) s1 ->
+               exists s2, initial_state (SC.sem prog) s2 /\ match_states s1 s2.
+
+  (* TODO this goes with r both nat or int, where is the type checking??!! *)
+  Axiom match_final_states:
+    forall s1 s2 (r:nat),
+      match_states s1 s2 ->
+      final_state (IC.sem tprog) s1 r ->
+      final_state (SC.sem prog) s2 r.
+  (* TODO this should be defined like above, pulling definitions from the
+     semantics but now there is a problem with nat and int *)
+  (* Axiom match_final_states: *)
+  (*   forall s1 s2 (r:int), *)
+  (*     match_states s1 s2 -> *)
+  (*     IC.final_state2 s1 r -> *)
+  (*     SC.final_state2 s2 r. *)
+
+  Axiom simulation:
+    forall s1 t s1', Step (IC.sem tprog) s1 t s1' ->
+                     forall s2, match_states s1 s2 ->
+                      exists s2', Step (SC.sem prog) s2 t s2' /\ match_states s1' s2'.
+
+
+  Axiom transl_program_correct:
+    forward_simulation (IC.sem tprog) (SC.sem prog).
+  (* TODO this works with match_final_states defined more general *)
+  (* Proof. *)
+  (*   eapply forward_simulation_step.  *)
+  (*   eexact match_initial_states. *)
+  (*   eexact match_final_states. *)
+  (*   eexact simulation. *)
+  (* Qed. *)
+End Cbs.
+
+Module Pbs.
+
+Variable psi: Program.interface.
+(* Definition SPstate := state (SP.sem prog psi). *)
+(* Definition IPstate := state (IP.sem tprog psi). *)
+(* Definition ICinitial_state := initial_state (IC.sem tprog). *)
+(* Definition SCinitial_state := initial_state (SC.sem prog). *)
+
+(* TODO why was this definition requiring to introduce an 'exists' in the proof
+while the other doesn't?! *)
+(* Definition SPinitial_state *)
+(*            (p: Source.program) (ctx: Program.interface) *)
+(*            (ps: SP.state) : Prop := *)
+(*   forall cs, SC.initial_state p cs -> *)
+(*              SPpartialize_state ctx cs ps. *)
+
+Inductive match_states: IP.state -> SP.state -> Prop :=
+| match_states_program:
+    forall ics scs ips sps,
+      Cbs.match_states ics scs ->
+      sps = SP.partialize_state psi scs ->
+      ips = IP.partialize_state psi ics ->
+      match_states ips sps
+| match_states_context:
+    forall (C:Component.id) (m:Memory.t) ic_stack sc_stack ip_stack sp_stack,
+      Cbs.match_stacks ic_stack sc_stack ->
+      IP.partialize_stack psi ic_stack ip_stack ->
+      SP.partialize_stack psi sc_stack sp_stack ->
+      match_states (IP.CC (C, ip_stack, m) IP.Normal)
+                   (SP.CC (C, sp_stack, m) SP.Normal).
+
+(* TODO we should use the match_states inside the simulation to make the proof more general, but compcert's simulations have a match_states with index, not sure how to make that work *)
+Lemma transl_initial_states:
+  forall S, IP.initial_state2 tprog psi S ->
+  exists R, SP.initial_state2 prog psi R /\ match_states S R.
+Proof.
+  intros S HinitS.
+  destruct Cbs.transl_program_correct as [index order Cmatch_states props].
+  destruct HinitS as [ips ics [h1 h2]].
+  specialize (Cbs.match_initial_states ics h1). intro Cmatch_initial_states.
+  destruct Cmatch_initial_states as [scs [h3 h4]].
+  exists (SP.partialize_state psi scs).
+  split.
+  - econstructor.
+    split.
+    apply h3.
+    auto.
+  - econstructor.
+    apply h4.
+    auto.
+    auto.
+Qed.
+
+Lemma transl_final_states:
+  forall (ips:IP.state) (sps:SP.state) (r:int),
+    match_states ips sps -> IP.final_state2 psi ips r -> SP.final_state2 psi sps r.
+Proof.
+  intros ips sps r H1 H2.
+  destruct H1.
+  destruct H2.
+  subst.
+  destruct (SP.final_state_intro psi sps r scs).
+
+  destruct H2.
+  subst.  
+  -
+    specialize (Cbs.match_final_states ics scs r H).
+    intro H3.
+
+    subst.
+    specialize (IP.final_state_intro psi ips r).
+  intro H4.
+  destruct h2.
+  
+
+    apply Cbs.match_final_states in H.
+  specialize (IP.final_state_intro psi ips r).
+  intro H.
+  subst.
+
+  intro H.
+
+  destruct h2 as [ics h3].
+  destruct (H ics). h3 H0).
+                          specialize (H ics h3 H0).
+  destruct H as [].
+  subst.
+  - apply Cbs.match_final_states with (r:=r) in H.
+    econstructor.
+    split.
+    apply H.
+    auto.
+    Check IP.IC.final_state2.
+    (* IP.IC.final_state *)
+    (*  : GlobalEnv.global_env -> IP.IC.state -> nat -> Prop *)
+
+    Check final_state (IC.sem tprog).
+    (* final_state (IC.sem tprog) *)
+    (*      : state (IC.sem tprog) -> int -> Prop *)
+
+    apply h3.
+
+
+
+Let ge : Source.GlobalEnv.global_env := Source.GlobalEnv.init_genv prog.
+Let tge : Intermediate.GlobalEnv.global_env := Intermediate.GlobalEnv.init_genv tprog.
+
+
+Axiom transl_step_correct:
+  forall s1 t s1', IPS.step psi tge s1 t s1' ->
+  forall s2, match_states s1 s2 ->
+  exists s2', SPS.kstep psi ge s2 t s2' /\ match_states s1' s2'.
+
+(* S simulates I, L1=IPS.sem L2=SPS.sem *)
+Theorem transl_program_correct:
+  forward_simulation (IPS.sem tprog psi) (SPS.sem prog psi).
+Proof.
+  eapply forward_simulation_step.
+  (* apply senv_preserved. *)
+  eexact transl_initial_states.
+  eexact transl_final_states.
+  eexact transl_step_correct.
+Qed.
